starting implementation with propagate queue

Weidenbach_Book/CDCL_Two_Watched_Literals_Implementation.thy
@@ -7,38 +7,87 @@ section \<open>Implementation for 2 Watched-Literals\<close>
 theory CDCL_Two_Watched_Literals_Implementation
 imports CDCL_Two_Watched_Literals_Invariant
 begin
+datatype 'v candidate =
+  Prop_Or_Conf
+    (prop_queue: "('v, nat, 'v twl_clause) marked_lit list")
+    (conflict: "'v twl_clause option")
 
 datatype 'v twl_state_cands =
   TWL_State_Cand (twl_state: "'v twl_state")
-    (propa_cand: "('v literal \<times> 'v twl_clause) list")
-    (confl_cand: "'v twl_clause literal")
+    (cand: "'v candidate")
+
+fun find_earliest_conflict :: "('v, nat, 'v twl_clause) marked_lits \<Rightarrow>
+  'v twl_clause \<Rightarrow> 'v twl_clause option \<Rightarrow> 'v twl_clause" where
+"find_earliest_conflict _ C None = C" |
+"find_earliest_conflict [] C _ = C" |
+"find_earliest_conflict (L # M) C (Some D) =
+  (case (M \<Turnstile>a mset (raw_clause C), \<not>M\<Turnstile>a mset (raw_clause D)) of
+    (True, True) \<Rightarrow> find_earliest_conflict M C (Some D)
+  | (False, True) \<Rightarrow> D
+  | (True, False) \<Rightarrow> C
+  | _ \<Rightarrow> C)"
 
 text \<open>While updating the clauses, there are several cases:
   \<^item> @{term L} is not watched and there is nothing to do;
   \<^item> there is a literal to be watched: there are swapped;
   \<^item> there is no literal to be watched, the other literal is not assigned: the clause
-  is a propagate candidate;
+  is a propagate or a conflict candidate;
   \<^item> there is no literal to be watched, but the other literal is true: there is nothing to
   do;
   \<^item> there is no literal to be watched, but the other literal is false: the clause is a
   conflict candidate.\<close>
-definition
-  rewatch_nat_cand ::
-  "'v literal \<Rightarrow> 'v twl_state \<Rightarrow> 'v twl_clause \<Rightarrow>
-     'v twl_clause \<times> ('v literal \<times> 'v twl_clause) option \<times> 'v twl_clause option"
+fun
+  rewatch_nat_cand_single_clause ::
+  "'v literal \<Rightarrow> ('v, nat, 'v twl_clause) marked_lits \<Rightarrow> 'v twl_clause \<Rightarrow>
+    'v twl_clause list \<times> 'v candidate \<Rightarrow>
+     'v twl_clause list  \<times> 'v candidate"
 where
-  "rewatch_nat_cand L S C =
-   (if - L \<in> set (watched C) then
-      case filter (\<lambda>L'. L' \<notin> set (watched C) \<and> - L' \<notin> insert L (lits_of_l (trail S)))
-         (unwatched C) of
-        [] \<Rightarrow> (if trail S \<Turnstile>as CNot (mset (remove1 L (watched C)))
-          then (C, None, Some C)
-          else if set (remove1 L (watched C)) \<subseteq> set (map lit_of (trail S))
-            then (C, None, None)
-            else (C, Some (L, C), None))
-      | L' # _ \<Rightarrow>
-        (TWL_Clause (L' # remove1 (-L) (watched C)) (-L # remove1 L' (unwatched C)), None, None)
-    else
-      (C, None, None))"
+"rewatch_nat_cand_single_clause L M C (Cs, Ks) =
+  (if - L \<in> set (watched C) then
+     case filter (\<lambda>L'. L' \<notin> set (watched C) \<and> - L' \<notin> insert L (lits_of_l M))
+        (unwatched C) of
+       [] \<Rightarrow>
+         (if M @ prop_queue Ks \<Turnstile>as CNot (mset (remove1 (-L) (watched C)))
+         then (C # Cs, Prop_Or_Conf (prop_queue Ks)
+           (Some (find_earliest_conflict M C (conflict Ks))))
+         else
+           if set (remove1 (-L) (watched C)) \<subseteq> lits_of_l (M @ prop_queue Ks)
+             (* it contains at most one variable, so... *)
+           then (C # Cs, Ks)
+           else (C # Cs, Prop_Or_Conf (Propagated L C # prop_queue Ks) (conflict Ks)))
+     | L' # _ \<Rightarrow>
+       (TWL_Clause (L' # remove1 (-L) (watched C)) (-L # remove1 L' (unwatched C)) # Cs, Ks)
+  else
+    (C # Cs, Ks))"
 
+declare rewatch_nat_cand_single_clause.simps[simp del]
+
+fun rewatch_nat_cand :: "'a literal \<Rightarrow> 'a twl_state_cands \<Rightarrow> 'a twl_state_cands"  where
+"rewatch_nat_cand L (TWL_State_Cand S Ks) =
+  (let update = \<lambda>Cs Ks. foldr (rewatch_nat_cand_single_clause L (raw_trail S)) Cs ([], Ks);
+    (N, K) = update (raw_init_clss S) Ks;
+    (U, K') = update (raw_learned_clss S) K in
+  TWL_State_Cand
+    (TWL_State (raw_trail S) N U (backtrack_lvl S) (raw_conflicting S))
+    K')"
+
+lemma length_Suc_Suc_0: "length S = 2 \<longleftrightarrow> (\<exists>a b. S = [a, b])"
+  sorry
+lemma XX: "set_mset (remove1_mset (- lit_of l) (mset W)) = set (remove1 (-lit_of L) W)"
+apply auto
+sorry
+lemma
+  assumes
+    undef: "undefined L M" and
+    "wf_twl_cls M C" and
+    n_d: "no_dup (M @ prop_queue Ks)"
+  shows "no_dup (prop_queue (snd (rewatch_nat_cand_single_clause L M C (Cs, Ks))))"
+  unfolding rewatch_nat_cand_single_clause.simps
+  apply (cases Ks; cases C)
+  apply (rename_tac M' Confl W UW)
+  using undef n_d apply (auto split: list.splits simp: atm_of_eq_atm_of filter_empty_conv
+    true_annots_true_cls_def_iff_negation_in_model lits_of_def length_Suc_Suc_0 image_Un
+    simp add: XX)
+
+  oops
 end
